Update: acc の定義を改善

theories/Relation.v
@@ -40,66 +40,59 @@ Definition rel_dsum {A : Type} (R : A -> A -> Type) (P : A -> Type)
 
 (** ** Well foundness *)
 
-(** [A] の関係 [R] は [x : A] において整礎である。 *)
-Inductive acc (A : Type) (R : A -> A -> Type) (x : A) : Type
-  :=
-  | mk_acc : (forall xp : A, R xp x -> acc A R xp) -> acc A R x
-  .
+Section Acc .
 
-Definition acc_case_nodep
-  (A : Type) (R : A -> A -> Type) (x : A) (P : Type)
-  (case_mk_acc : (forall xp : A, R xp x -> acc A R xp) -> P)
-  (H : acc A R x) : P
-  := match H with mk_acc _ _ _ Hp => case_mk_acc Hp end .
+  Variable A : Type .
+  Variable R : A -> A -> Type .
 
-Definition acc_case
-  (A : Type) (R : A -> A -> Type) (x : A) (P : acc A R x -> Type)
-  (case_mk_acc
-     : forall Hp : (forall xp : A, R xp x -> acc A R xp), P (mk_acc A R x Hp))
-  (H : acc A R x) : P H
-  := match H with mk_acc _ _ _ Hp => case_mk_acc Hp end .
+  (** [A] の関係 [R] は [x : A] において整礎である。 *)
+  Inductive acc (x : A) : Type
+    :=
+    | mk_acc : (forall xp, R xp x -> acc xp) -> acc x
+    .
 
-Definition acc_rec
-  (A : Type) (R : A -> A -> Type) (P : A -> Type)
-  (case_mk_acc : forall x : A, (forall xp : A, R xp x -> P xp) -> P x)
-  (x : A) (H : acc A R x) : P x .
-Proof.
- revert x H .
- refine (fix go (x : A) (H : acc A R x) {struct H} : P x := _) .
- refine (acc_case_nodep A R x (P x) _ H) .
- -
-  refine (fun Hp => _) .
-  refine (case_mk_acc x _) .
-  refine (fun xp xpR => _) .
-  exact (go xp (Hp xp xpR)) .
-Defined.
+  Definition acc_case_nodep
+    (x : A) (P : Type)
+    (case_mk_acc : (forall xp, R xp x -> acc xp) -> P)
+    (H : acc x) : P
+    := match H with mk_acc _ Hp => case_mk_acc Hp end .
 
-Definition acc_rect
-  (A : Type)
-  (R : A -> A -> Type)
-  (P : forall x : A, acc A R x -> Type)
-  (case_mk_acc
-     : forall (x  : A)
-              (Hp : forall xp : A,
-                                R xp x ->
-                                acc A R xp),
-              (forall (xp  : A)
-                      (xpR : R xp x),
-                             P xp (Hp xp xpR)) ->
-               P x (mk_acc A R x Hp))
-  (x : A)
-  (H : acc A R x)
-     : P x H .
-Proof.
- revert x H .
- refine (fix go (x : A) (H : acc A R x) {struct H} : P x H := _) .
- refine (acc_case A R x (P x) _ H) .
- -
-  refine (fun Hp => _) .
-  refine (case_mk_acc x Hp _) .
-  refine (fun xp xpR => _) .
-  exact (go xp (Hp xp xpR)) .
-Defined.
+  Definition acc_case
+    (x : A) (P : acc x -> Type)
+    (case_mk_acc : forall Hp , P (mk_acc x Hp))
+    (H : acc x) : P H
+    := match H with mk_acc _ Hp => case_mk_acc Hp end .
+
+  Definition acc_rec
+    (P : A -> Type)
+    (case_mk_acc : forall x, (forall xp, R xp x -> P xp) -> P x)
+    (x : A) (H : acc x) : P x .
+  Proof.
+   revert x H .
+   refine (fix go (x : A) (H : acc x) {struct H} : P x := _) .
+   refine (acc_case_nodep x (P x) _ H) .
+   refine (fun Hp => _) .
+   refine (case_mk_acc x _) .
+   refine (fun xp xpR => _) .
+   exact (go xp (Hp xp xpR)) .
+  Defined.
+
+  Definition acc_rect
+    (P : forall x, acc x -> Type)
+    (case_mk_acc
+       : forall x Hp, (forall xp xpR, P xp (Hp xp xpR)) -> P x (mk_acc x Hp))
+    (x : A) (H : acc x) : P x H .
+  Proof.
+   revert x H .
+   refine (fix go (x : A) (H : acc x) {struct H} : P x H := _) .
+   refine (acc_case x (P x) _ H) .
+   refine (fun Hp => _) .
+   refine (case_mk_acc x Hp _) .
+   refine (fun xp xpR => _) .
+   exact (go xp (Hp xp xpR)) .
+  Defined.
+
+End Acc.
 
 Arguments acc {_} _ _ .
 Arguments mk_acc {_ _ _} _ .
